mppa_k1c/PostpassSchedulingOracle.ml
@@ -1,0 +1,18 @@
+open Asmblock
+
+let bundlize_label l =
+  match l with
+  | [] -> []
+  | l -> [{ header = l; body = []; exit = None }]
+
+let rec bundlize_basic l =
+  match l with
+  | [] -> []
+  | b :: l -> { header = []; body = [b]; exit = None } :: bundlize_basic l
+
+let bundlize_exit e =
+  match e with
+  | Some e -> [{ header = []; body = []; exit = Some e }]
+  | None -> []
+
+let schedule (bb : bblock) : bblock list = bundlize_label bb.header @ bundlize_basic bb.body @ bundlize_exit bb.exit
