mppa_k1c/Asmgen.v
@@ -17,6 +17,7 @@
 
 Require Import Integers.
 Require Import Mach Asm Asmblock Asmblockgen Machblockgen.
+Require Import PostpassScheduling.
 Require Import Errors.
 
 Local Open Scope error_monad_scope.
@@ -24,7 +25,8 @@ Local Open Scope error_monad_scope.
 Definition transf_program (p: Mach.program) : res Asm.program :=
   let mbp := Machblockgen.transf_program p in
   do abp <- Asmblockgen.transf_program mbp;
-  OK (Asm.transf_program abp).
+  do abp' <- PostpassScheduling.transf_program abp;
+  OK (Asm.transf_program abp').
 
 Definition transf_function (f: Mach.function) : res Asm.function :=
   let mbf := Machblockgen.transf_function f in
